Bedrock/Platform/Facade/examples/TuplesF.v
@@ -111,12 +111,12 @@ Definition functional {A} (ts : GenericTuples A) :=
   forall t1 t2, Ensembles.In _ ts t1 -> Ensembles.In _ ts t2
                 -> elementIndex t1 = elementIndex t2 -> t1 = t2.
 
-Definition keepEq {A B} (EQ: A -> B -> Prop) (ts : GenericTuples A) (key: W) (k : B) : GenericTuples A :=
+Definition keepEq {A B} (EQ: A -> B -> Prop) (default : A) (ts : GenericTuples A) (key: W) (k : B) : GenericTuples A :=
   fun tup => Ensembles.In _ ts tup /\
-          match List.nth_error (indexedElement tup) (wordToNat key) with
-          | Some k0 => EQ k0 k
-          | None => False
-          end.
+          EQ match List.nth_error (indexedElement tup) (wordToNat key) with
+             | Some k0 => k0
+             | None => default
+             end k.
 
 Definition tupl := GenericTuple W.
 Definition tuples := GenericTuples W.
